Behaviour, Labels ....

Label.v
@@ -2,8 +2,8 @@ Definition Location := nat.
 Definition Value := nat.
 
 Class LabelClass (L : Type):Type := {
-  lab_loc : L -> option Location;
-  lab_val : L -> option Value; 
+  lab_loc : L -> Location;
+  lab_val : L -> Value; 
   is_r : L -> Prop;
   is_w : L -> Prop;
 }. 
