Executions.v
@@ -49,20 +49,36 @@ Definition poloc {Label: Type} {LabelProof: LabelClass Label} (exec:Execution) :
 Definition poimm {Label: Type} {LabelProof: LabelClass Label} (exec:Execution) : relation Event  := 
     fun e1 e2 =>  ((po exec) e1 e2) /\ ~(exists e3, ((po exec) e1 e3) /\ ((po exec) e3 e2)).
 
-
+(* Expresses that an mo relation can only exist between two independent writes on the same location. *)
 Definition well_formed_mo {Label: Type} {LabelProof: LabelClass Label} (exec:Execution) :Prop := 
-    forall (e1 e2:Event), (mo exec) e1 e2 -> both_write e1 e2 /\ same_loc e1 e2. 
+    forall (e1 e2:Event), (mo exec) e1 e2 -> both_write e1 e2 /\ same_loc e1 e2 /\ e1 <> e2. 
 
+(* Expresses that an rf relation can only exist between a write and a read on the same location, 
+   with the same value, and that a read can only be from a single write *)
 Definition well_formed_rf {Label: Type} {LabelProof: LabelClass Label} (exec:Execution) :Prop := 
     forall (w r:Event), (rf exec) w r -> is_w (event_label w) /\ is_r (event_label r)
                                          /\ same_loc w r 
                                          /\ same_val w r 
                                          /\ forall (w0:Event), is_w (event_label w0) -> (rf exec) w0 r -> w0 = w.   
 
+(* Expresses that a read modify write relation can only exist between immediate reads and writes on the same location. *)
 Definition well_formed_rmw {Label: Type} {LabelProof: LabelClass Label} (exec:Execution) :Prop := 
     forall (r w:Event), (rmw exec) r w -> is_r (event_label r) /\ is_w (event_label w)
                                           /\ (poimm exec) r w
                                           /\ same_loc r w. 
 
+(* Predicate to express well-formedness on an execution graph. *)
 Definition well_formed {Label: Type} {LabelProof: LabelClass Label} (exec:Execution) :Prop := 
     well_formed_mo exec /\ well_formed_rf exec /\ well_formed_rmw exec. 
+
+(* Define atomicity and coherence axioms because they are generic across the two itegrations *)
+(* Hahn gives us a ⨾ for relation composition (haskell . but better) *)
+
+Definition Behaviour {Label: Type} {LabelProof: LabelClass Label} (X : Execution) : Location * Value -> Prop :=
+  fun '(l,v) =>
+    exists e, 
+      is_w (event_label e) /\
+      lab_loc (event_label e) = l /\
+      lab_val (event_label e) = v /\ 
+      ~(exists (e': Event), (X.(mo) e e')). 
+      
