LabelArm.v
@@ -1,0 +1,33 @@
+(* ob = (bob ∪ rfe ∪ moe ∪ fre)+ *)
+(* bob = ((R_acq_pc ; po) ∪ (po ; W_rel))*)
+
+(* ob is irreflexive *)
+
+From RelAcqProof Require Import Label. 
+
+Inductive LabelArm := 
+| W_Rel (loc:Location) (val:Value)
+| R_Acq_Pc (loc:Location) (val:Value). 
+
+(* Instance LabelClassArm: LabelClass LabelArm.  *)
+Instance LabelClassArm: LabelClass LabelArm := {
+    lab_loc l := match l with
+                | W_Rel loc _ => loc 
+                | R_Acq_Pc loc _ => loc 
+                end;
+      
+    lab_val l := match l with
+                | W_Rel _ val => val 
+                | R_Acq_Pc _ val => val 
+                end;
+
+    is_r l := match l with
+                | W_Rel _ _ => True 
+                | R_Acq_Pc _ _ => False 
+                end;
+
+    is_w l := match l with
+                | W_Rel _ _ => False 
+                | R_Acq_Pc _ _ => True 
+                end;
+}. 
